lawyer/nonblocking/logrel/fundamental.v
@@ -1,0 +1,642 @@
+(* From iris.program_logic Require Import lifting ectx_lifting. *)
+(* From iris.program_logic Require Export weakestpre. *)
+
+From iris.proofmode Require Import proofmode.
+From lawyer.nonblocking.logrel Require Export persistent_pred logrel.
+From lawyer.nonblocking Require Export pwp. 
+From iris.base_logic Require Import invariants.
+From iris.prelude Require Import options.
+From heap_lang Require Import heap_lang_defs sswp_logic.
+
+
+Section typed_interp.
+  Context {Σ: gFunctors}
+    (* {iG: irisG heap_lang LoopingModel Σ} *)
+    {hG: heap1GS Σ}
+    {invG: invGS_gen HasNoLc Σ}
+  .
+
+  Let iG := irisG_looping HeapLangEM (lG := hG).
+  Existing Instance iG. 
+  
+  Notation D := (persistent_predO val (iPropI Σ)).
+
+  Lemma subst_env_var x vs:
+    subst_env vs (Var x) = from_option Val (Var x) (vs !! x).
+  Proof using.
+    rewrite /subst_env.
+
+    set (P := fun (e: expr heap_lang) (mp: gmap string (val heap_lang)) =>
+                e = from_option Val (Var x) (mp !! x)).
+    enough (P (map_fold subst (Var x) vs) vs).
+    { done. }
+
+    apply map_fold_weak_ind; clear vs. 
+    { done. }
+    subst P. simpl. intros s v vs e NIN ->.
+    rewrite insert_union_singleton_l. rewrite lookup_union.
+    rewrite utils_maps.lookup_map_singleton.
+
+    destruct decide as [-> | NEQ]. 
+    { simpl. rewrite NIN. simpl. by rewrite decide_True. }
+    rewrite option_union_left_id.
+    destruct (vs !! x) eqn:XTH.
+    - simpl. done.
+    - simpl. by rewrite decide_False.
+  Qed.
+
+  Lemma logrel_var x : ⊢ logrel (Var x).
+  Proof.
+    iIntros "!#" (vs τ) "Henv".
+    rewrite subst_env_var /interp_expr. 
+    destruct (vs !! x) eqn:XTH; simpl. 
+    - iApply wp_value.
+      iApply interp_env_Some_l; done.
+    - admit. 
+  Admitted.
+
+  (* Lemma logrel_lit_noloc (v: base_lit) *)
+  (*   (NOLOC: forall l, v ≠ LitLoc l): *)
+  (*   ⊢ logrel (LitV v). *)
+
+  (* Lemma logrel_unit : ⊢ logrel UnitV. *)
+  (* Proof. *)
+  (*   iIntros "!#" (vs) "Henv". *)
+  (*   rewrite /interp_expr. *)
+  (*   simpl.  *)
+  (*   iApply wp_value. rewrite interp_unfold. done. *)
+  (* Qed. *)
+
+  (* Lemma logrel_nat n : ⊢ logrel (#n n). *)
+  (* Proof. *)
+  (*   iIntros "!#" (vs) "Henv". *)
+  (*   (* Unset Printing Notations. *) *)
+  (*   iApply wp_value. rewrite interp_unfold /=; done. *)
+  (* Qed. *)
+
+  (* Lemma logrel_bool b : ⊢ logrel (#♭ b). *)
+  (* Proof. iIntros "!#" (vs) "Henv"; iApply wp_value; rewrite interp_unfold /=; done. Qed. *)
+
+  (* Lemma logrel_loc l: ⊢ logrel (Loc l). *)
+
+  Lemma bin_op_eval_inv op a b r
+    (EVAL: bin_op_eval op a b = Some r):
+    (op = EqOp /\ vals_compare_safe a b /\ r = LitV $ LitBool $ bool_decide (a = b)) \/
+    (exists na nb vr, a = LitV $ LitInt na /\ b = LitV $ LitInt nb /\ r = LitV vr /\
+                 ((exists i, vr = LitInt i) \/ (exists b, vr = LitBool b)) /\
+                 bin_op_eval_int op na nb = Some vr) \/
+    (exists ba bb br, a = LitV $ LitBool ba /\ b = LitV $ LitBool bb /\ r = LitV $ LitBool br /\
+                 bin_op_eval_bool op ba bb = Some $ LitBool br) \/
+    (exists la ob, a = LitV $ LitLoc la /\ b = LitV (LitInt ob) /\ 
+              r = LitV (LitLoc (la +ₗ ob))).
+  Proof using.
+    rewrite /bin_op_eval in EVAL.
+    destruct decide.
+    { subst. destruct decide; [| done].
+      left. inversion EVAL. subst. eauto. }
+    destruct a; try done.
+    destruct l; try done.
+    all: destruct b; (try done); destruct l; try done.
+    - apply fmap_Some in EVAL as (?&?&->).
+      right. left. do 3 eexists. repeat split; eauto.
+      destruct op; simpl in H; set_solver.      
+    - apply fmap_Some in EVAL as (?&?&->).
+      destruct op; simpl in H; set_solver.
+    - destruct l0; try done.
+      inversion EVAL. subst. eauto.
+      repeat right. eauto.
+  Qed.
+
+  Ltac inv_binop_eval H :=
+    apply bin_op_eval_inv in H as
+        [(-> & ? & ->) | [(?&?&?&->&->&->&[(?&->) | (?&->)]&?) | [(?&?&?&->&->&->&?) | (?&?&->&->&->)]]].
+
+  Lemma interp_binop_eval op n1 n2
+    (NOLOC: forall l, n1 ≠ LitV (LitLoc l)):
+    ⊢ from_option interp (⌜ True ⌝) (bin_op_eval op n1 n2).
+  Proof.
+    destruct (bin_op_eval op n1 n2) eqn:EVAL; [| done]. simpl.
+    inv_binop_eval EVAL.
+    5: set_solver.
+    all: by rewrite interp_unfold. 
+  Qed.
+
+  Definition valid_base_lit (v: base_lit) : Prop :=
+    match v with
+    | LitInt _ | LitBool _ | LitUnit => True
+    | LitLoc _ | LitProphecy _ | LitPoison => False
+  end.
+
+  (* an adversary proram is any program with no hard-coded locations.
+     TODO: currently we also exclude prophecies, seems reasonable? *)
+  Fixpoint valid_adversary (e : expr heap_lang) : Prop :=
+    match e with
+    | Val v => valid_val v
+    | Var _ | ChooseNat => True
+    | Rec _ _  e | UnOp _ e | Fst e | Snd e |
+      InjL e | InjR e | Fork e | Load e
+      => valid_adversary e
+    | App e1 e2 | Pair e1 e2 | BinOp _ e1 e2 |
+      AllocN e1 e2 | Store e1 e2 | FAA e1 e2
+      => valid_adversary e1 /\ valid_adversary e2
+    | If e0 e1 e2 | Case e0 e1 e2 | CmpXchg e0 e1 e2
+      => valid_adversary e0 /\ valid_adversary e1 /\ valid_adversary e2
+    end
+  with valid_val (v: val heap_lang) : Prop :=
+    match v with
+    | LitV b => valid_base_lit b
+    | RecV _ _ e => valid_adversary e
+    | PairV v1 v2 => valid_val v1 /\ valid_val v2
+    | InjLV v | InjRV v => valid_val v
+    end.
+
+  Lemma subst_env_binop vs op e1 e2:
+    subst_env vs (BinOp op e1 e2) = BinOp op (subst_env vs e1) (subst_env vs e2).
+  Proof using.
+    rewrite /subst_env.
+    generalize dependent e1. generalize dependent e2. generalize dependent op. 
+    pattern vs. apply map_first_key_ind. 
+    { intros. by rewrite !map_fold_empty. }
+    intros s v m NIN FKEY IH op e1 e2.
+    rewrite !map_fold_insert_first_key; auto.
+    by rewrite IH.
+  Qed.
+
+  (* TODO: remove duplicates*)
+  From iris.proofmode Require Import coq_tactics.
+  From heap_lang Require Import tactics. 
+
+Lemma tac_wp_bind
+  K Δ s E Φ e f :
+  f = (λ e, fill K e) → (* as an eta expanded hypothesis so that we can `simpl` it *)
+  envs_entails Δ (WP e @ s; E {{ v, WP f (Val v) @ s; E {{ Φ }} }})%I →
+  envs_entails Δ (WP fill K e @ s; E {{ Φ }}).
+Proof. rewrite envs_entails_unseal=> -> ->. by apply: wp_bind. Qed.
+
+Ltac wp_bind_core K :=
+  lazymatch eval hnf in K with
+  | [] => idtac
+  | _ => eapply (tac_wp_bind K); [simpl; reflexivity|reduction.pm_prettify]
+  end.
+
+Tactic Notation "wp_bind" open_constr(efoc) :=
+  iStartProof;
+  lazymatch goal with
+  | |- envs_entails _ (wp ?s ?E ?locale ?e ?Q) =>
+      first [ reshape_expr e ltac:(fun K e' => unify e' efoc; wp_bind_core K)
+            | fail 1 "wp_bind: cannot find" efoc "in" e ]
+  | _ => fail "wp_bind: not a 'wp'"
+  end.
+
+  (* Goal forall (e1 e2: expr) (op: bin_op) (mp: gmap string val), False. *)
+  (*   intros e1 e2 op vs. *)
+  (*   (* Set Ltac Debug.  *) *)
+  (*   reshape_expr (BinOp op (subst_env vs e1) (subst_env vs e2)) ltac:(fun K e' => unify e' (subst_env vs e2); wp_bind_core K).  *)
+
+  (* TODO: move? try to unify with sswp_MU_wp_fupd  *)
+  Lemma sswp_pwp s E E' τ e Φ
+    (NVAL: language.to_val e = None):
+    (|={E,E'}=> sswp s E' e (λ e', ▷ |={E',E}=> pwp s E τ e' Φ)%I) -∗
+    pwp s E τ e Φ.
+  Proof using.
+    rewrite /pwp wp_unfold /wp_pre.
+    iIntros "Hsswp". rewrite NVAL. 
+    iIntros (extr atr K tp1 tp2 σ1 Hvalid Hζ Hextr) "Hσ".
+    iMod "Hsswp" as "foo".
+    rewrite /sswp. rewrite NVAL.
+    iSimpl in "Hσ".
+    iSpecialize ("foo" with "[$]").
+    iMod "foo" as (Hs) "Hsswp".
+    red in Hextr. rewrite Hextr. 
+    iModIntro. iSplit.
+    { iPureIntro. by rewrite Hextr in Hs. }
+    iIntros (e2 σ2 efs Hstep).
+    iDestruct ("Hsswp" with "[//]") as "Hsswp".
+    iApply (step_fupdN_le 2); [| done| ].
+    { pose proof (trace_length_at_least extr). lia. }
+    simpl.
+    iApply (step_fupd_wand with "Hsswp").
+    iIntros ">(Hσ & HMU & ->)".
+    iApply fupd_mask_intro; [set_solver| ]. iIntros "CLOS' !> !>".
+    iMod "CLOS'" as "_". iMod "HMU". iModIntro.
+    iExists tt, tt. by iFrame.
+  Qed.
+
+  (* (* TODO: probably can strenghten it *) *)
+  (* Lemma fill_item_fill_comm_weak K i e: *)
+  (*   exists i' e', fill K (fill_item i e) = fill_item i' e'. *)
+  (* Proof using. *)
+  (*   generalize dependent i. generalize dependent e. induction K; eauto. *)
+  (* Qed. *)
+
+  Lemma foldl_foldr_rev {A B : Type} (f : B → A → B) (b : B) (la : list A):
+    foldl f b la = foldr (flip f) b (rev la). 
+  Proof using.
+    generalize dependent b. induction la.
+    { done. }
+    simpl. intros. rewrite IHla.
+    by rewrite foldr_app.
+  Qed.
+        
+  (* Lemma binop_imm_no_fill op v1 v2: *)
+  (*   ¬ exists i K e, BinOp op (Val v1) (Val v2) = fill (i :: K) e. *)
+  (* Proof using. *)
+  (*   simpl. red. intros (i&K&e&FILL). *)
+  (*   generalize dependent i. generalize dependent e. *)
+  (*   induction K. *)
+  (*   { intros. simpl in FILL. *)
+  (*     destruct i; simpl in FILL; try congruence. *)
+  (*     - inversion FILL. subst. *)
+  (*       admit. *)
+  (*     - inversion FILL. subst.  *)
+
+  (* TODO: move? *)
+  Lemma binop_srav op v1 v2:
+    sub_redexes_are_values (BinOp op (Val v1) (Val v2)).
+  Proof using.
+    red. simpl. intros. 
+    rewrite /fill in H.
+    rewrite foldl_foldr_rev in H. simpl in H.
+    destruct (rev K) eqn:RR.
+    { eapply (@f_equal _ _ length) in RR.
+      rewrite length_rev /= in RR.
+      destruct K; simpl in *; done. }
+    clear RR. simpl in H.
+    rewrite -(rev_involutive l) in H. rewrite -foldl_foldr_rev in H.
+    replace (foldl (flip fill_item) e' (rev l)) with (fill (rev l) e') in H by done.
+    remember (fill (rev l) e') as e''.
+    assert (to_val e'' = None).
+    { subst.
+      destruct (to_val (fill _ _)) eqn:VV; [| done].
+      apply to_val_fill_some in VV as (?&->). done. }
+    clear Heqe''.       
+    destruct e; simpl in H; try congruence.
+    all: inversion H; subst; done.
+  Qed.
+
+  Lemma logrel_nat_binop op e1 e2 : logrel e1 -∗ logrel e2 -∗ logrel (BinOp op e1 e2).
+  Proof.
+    iIntros "#IH1 #IH2 !#" (vs τ) "#Henv"; rewrite /interp_expr /=.
+    rewrite subst_env_binop.
+    rewrite {3}/pwp.
+
+    (* Set Ltac Backtrace.  *)
+    (* reshape_expr (BinOp op (subst_env vs e1) (subst_env vs e2)) ltac:(fun K e' => unify e' efoc; wp_bind_core K).  *)
+    (* Set Ltac Debug.  *)
+    (* reshape_expr (BinOp op (subst_env vs e1) (subst_env vs e2)) ltac:(fun K e' => unify e' (subst_env vs e2); wp_bind_core K). *)
+    (* TODO: fix wp_bind tactic *)
+
+    iApply (wp_bind [BinOpRCtx _ _]).
+    iApply wp_wand; [by iApply "IH2"| ].
+    iIntros (v2) "#Hv2 /=".
+    iApply (wp_bind [BinOpLCtx _ _]).
+    iApply wp_wand; [by iApply "IH1"| ].
+    iIntros (v1) "#Hv1 /=".
+
+    destruct (bin_op_eval op v1 v2) eqn:EVAL.
+    2: { iApply ectx_lifting.wp_lift_pure_head_stuck; try done.
+         { apply binop_srav. }        
+         intros. red. simpl. split; [done| ].
+         red. simpl. intros ??? STEP.
+         inversion STEP. subst. congruence. }
+
+    iApply sswp_pwp; [done| ].
+    iModIntro. iApply sswp_pure_step; [by apply EVAL| ].
+    iIntros "!> !>".
+    iApply wp_value.
+    
+    destruct (val_cases_nat v1) as [[? ->]|Hnn1], (val_cases_nat v2) as [[? ->]|Hnn2].
+    
+    destruct (val_cases_nat v1) as [[? ->]|Hnn1].
+    - destruct (val_cases_nat v2) as [[? ->]|Hnn2].
+      + iApply wp_pure_step_later; first done.
+        iNext; iIntros "_".
+        iApply wp_value.
+        iApply interp_binop_eval.
+      + iApply binop_stuck; auto.
+    - iApply binop_stuck; auto.
+  Qed.
+
+  Lemma logrel_pair e1 e2 : logrel e1 -∗ logrel e2 -∗ logrel (Pair e1 e2).
+  Proof.
+    iIntros "#IH1 #IH2 !#" (vs) "#Henv"; rewrite /interp_expr /=.
+    iApply (wp_bind (fill [PairLCtx _])).
+    iApply wp_wand; first by iApply "IH1".
+    iIntros (v1) "#Hv1 /=".
+    iApply (wp_bind (fill [PairRCtx _])).
+    iApply wp_wand; first by iApply "IH2".
+    iIntros (v2) "#Hv2 /=".
+    iApply wp_value.
+    rewrite {5}interp_unfold; simpl.
+    eauto 6.
+  Qed.
+
+  Lemma logrel_fst e : logrel e -∗ logrel (Fst e).
+  Proof.
+    iIntros "#IH !#" (vs) "#Henv"; rewrite /interp_expr /=.
+    iApply (wp_bind (fill [FstCtx])).
+    iApply wp_wand; first by iApply "IH".
+    iIntros (v) "#Hv /=".
+    destruct (val_cases_pair v) as [(? & ? & ->)|Hnp]; simpl.
+    - rewrite {2}interp_unfold; simpl.
+      iDestruct "Hv" as (? ?) "[>% [? ?]]"; simplify_eq.
+      iApply wp_pure_step_later; first done.
+      iNext; iIntros "_".
+      by iApply wp_value.
+    - iApply fst_stuck; done.
+  Qed.
+
+  Lemma logrel_snd e : logrel e -∗ logrel (Snd e).
+  Proof.
+    iIntros "#IH !#" (vs) "#Henv"; rewrite /interp_expr /=.
+    iApply (wp_bind (fill [SndCtx])).
+    iApply wp_wand; first by iApply "IH".
+    iIntros (v) "#Hv /=".
+    destruct (val_cases_pair v) as [(? & ? & ->)|Hnp]; simpl.
+    - rewrite {2}interp_unfold; simpl.
+      iDestruct "Hv" as (? ?) "[>% [? ?]]"; simplify_eq.
+      iApply wp_pure_step_later; first done.
+      iNext; iIntros "_".
+      by iApply wp_value.
+    - iApply snd_stuck; done.
+  Qed.
+
+  Lemma logrel_injl e : logrel e -∗ logrel (InjL e).
+  Proof.
+    iIntros "#IH !#" (vs) "#Henv"; rewrite /interp_expr /=.
+    iApply (wp_bind (fill [InjLCtx])).
+    iApply wp_wand; first by iApply "IH".
+    iIntros (v) "#Hv /=".
+    iApply wp_value.
+    rewrite {3}interp_unfold; simpl.
+    iLeft; eauto.
+  Qed.
+
+  Lemma logrel_injr e : logrel e -∗ logrel (InjR e).
+  Proof.
+    iIntros "#IH !#" (vs) "#Henv"; rewrite /interp_expr /=.
+    iApply (wp_bind (fill [InjRCtx])).
+    iApply wp_wand; first by iApply "IH".
+    iIntros (v) "#Hv /=".
+    iApply wp_value.
+    rewrite {3}interp_unfold; simpl.
+    iRight; eauto.
+  Qed.
+
+  Lemma logrel_case e0 e1 e2 : logrel e0 -∗ logrel e1 -∗ logrel e2 -∗ logrel (Case e0 e1 e2).
+  Proof.
+    iIntros "#IH0 #IH1 #IH2 !#" (vs) "#Henv"; rewrite /interp_expr /=.
+    iApply (wp_bind (fill [CaseCtx _ _])).
+    iApply wp_wand; first by iApply "IH0".
+    iIntros (v0) "#Hv0 /=".
+    destruct (val_cases_sum v0) as [[[? ->]|[? ->]]|Hns].
+    - rewrite {4}interp_unfold; simpl.
+      iDestruct "Hv0" as "[Hv0|Hv0]"; iDestruct "Hv0" as (?) "[>% ?]"; [simplify_eq|done].
+      iApply wp_pure_step_later; first done.
+      iNext; iIntros "_".
+      asimpl.
+      iApply ("IH1" $! (_ :: _)); rewrite interp_env_cons; iFrame "#".
+    - rewrite {4}interp_unfold; simpl.
+      iDestruct "Hv0" as "[Hv0|Hv0]"; iDestruct "Hv0" as (?) "[>% ?]"; [done|simplify_eq].
+      iApply wp_pure_step_later; first done.
+      iNext; iIntros "_".
+      asimpl.
+      iApply ("IH2" $! (_ :: _)); rewrite interp_env_cons; iFrame "#".
+    - iApply case_stuck; auto.
+  Qed.
+
+  Lemma logrel_if e0 e1 e2 : logrel e0 -∗ logrel e1 -∗ logrel e2 -∗ logrel (If e0 e1 e2).
+  Proof.
+    iIntros "#IH0 #IH1 #IH2 !#" (vs) "#Henv"; rewrite /interp_expr /=.
+    iApply (wp_bind (fill [IfCtx _ _])).
+    iApply wp_wand; first by iApply "IH0".
+    iIntros (v0) "#Hv0 /=".
+    destruct (val_cases_bool v0) as [[[] ->]|Hns].
+    - iApply wp_pure_step_later; first done.
+      iNext; iIntros "_".
+      iApply "IH1"; done.
+    - iApply wp_pure_step_later; first done.
+      iNext; iIntros "_".
+      iApply "IH2"; done.
+    - iApply if_stuck; auto.
+  Qed.
+
+  Lemma logrel_rec e : logrel e -∗ logrel (Rec e).
+  Proof.
+    iIntros "#IH !#" (vs) "#Henv"; rewrite /interp_expr /=.
+    iApply wp_value.
+    rewrite {2}interp_unfold; simpl.
+    iModIntro.
+    iLöb as "IHrec".
+    iIntros (v) "#Hv".
+    iApply wp_pure_step_later; first done.
+    iNext; iIntros "_".
+    asimpl.
+    change (Rec _) with (of_val (RecV e.[upn 2 (env_subst vs)])) at 2.
+    iApply ("IH" $! (_ :: _ :: vs)).
+    rewrite ?interp_env_cons; iFrame "Hv Henv".
+    rewrite {5}interp_unfold; simpl.
+    iModIntro; done.
+  Qed.
+
+  Lemma logrel_lam e : logrel e -∗ logrel (Lam e).
+  Proof.
+    iIntros "#IH !#" (vs) "#Henv"; rewrite /interp_expr /=.
+    iApply wp_value.
+    rewrite {2}interp_unfold; simpl.
+    iModIntro.
+    iIntros (v) "#Hv".
+    iApply wp_pure_step_later; first done.
+    iNext; iIntros "_".
+    asimpl.
+    iApply ("IH" $! (_ :: vs)).
+    rewrite ?interp_env_cons; iFrame "#".
+  Qed.
+
+  Lemma logrel_letin e1 e2 : logrel e1 -∗ logrel e2 -∗ logrel (LetIn e1 e2).
+  Proof.
+    iIntros "#IH1 #IH2 !#" (vs) "#Henv"; rewrite /interp_expr /=.
+    iApply (wp_bind (fill [LetInCtx _])).
+    iApply wp_wand; first by iApply "IH1".
+    iIntros (v) "#Hv /=".
+    iApply wp_pure_step_later; first done.
+    iNext; iIntros "_".
+    asimpl.
+    iApply ("IH2" $! (_ :: vs)).
+    rewrite ?interp_env_cons; iFrame "#".
+  Qed.
+
+  Lemma logrel_seq e1 e2 : logrel e1 -∗ logrel e2 -∗ logrel (Seq e1 e2).
+  Proof.
+    iIntros "#IH1 #IH2 !#" (vs) "#Henv"; rewrite /interp_expr /=.
+    iApply (wp_bind (fill [SeqCtx _])).
+    iApply wp_wand; first by iApply "IH1".
+    iIntros (v) "#Hv /=".
+    iApply wp_pure_step_later; first done.
+    iNext; iIntros "_".
+    iApply "IH2"; done.
+  Qed.
+
+  Lemma logrel_app e1 e2 : logrel e1 -∗ logrel e2 -∗ logrel (App e1 e2).
+  Proof.
+    iIntros "#IH1 #IH2 !#" (vs) "#Henv"; rewrite /interp_expr /=.
+    iApply (wp_bind (fill [AppLCtx _])).
+    iApply wp_wand; first by iApply "IH1".
+    iIntros (v1) "#Hv1 /=".
+    iApply (wp_bind (fill [AppRCtx _])).
+    iApply wp_wand; first by iApply "IH2".
+    iIntros (v2) "#Hv2 /=".
+    destruct (val_cases_fun v1) as [[[? ->]|[? ->]]|Hnf].
+    - rewrite {3}interp_unfold; simpl.
+      iApply "Hv1"; done.
+    - rewrite {3}interp_unfold; simpl.
+      iApply "Hv1"; done.
+    - iApply app_stuck; done.
+  Qed.
+
+  Lemma logrel_fork e : logrel e -∗ logrel (Fork e).
+  Proof.
+    iIntros "#IH !#" (vs) "#Henv"; rewrite /interp_expr /=.
+    iApply wp_fork.
+    iSplitR; iNext; first by rewrite {2}interp_unfold.
+    iApply wp_wand_l. iSplitL; [|iApply "IH"; auto]; auto.
+  Qed.
+
+  Lemma logrel_alloc e : logrel e -∗ logrel (Alloc e).
+  Proof.
+    iIntros "#IH !#" (vs) "#Henv"; rewrite /interp_expr /=.
+    iApply (wp_bind (fill [AllocCtx])).
+    iApply wp_wand; first by iApply "IH".
+    iIntros (v) "#Hv /=".
+    iApply wp_fupd.
+    iApply wp_stuck_weaken.
+    iApply wp_alloc; auto 1 using to_of_val.
+    iNext; iIntros (l) "Hl".
+    rewrite {3}interp_unfold /=.
+    iMod (inv_alloc _ with "[Hl]") as "HN";
+      [| iModIntro; iExists _; iSplit; trivial]; eauto.
+  Qed.
+
+  Lemma logrel_load e : logrel e -∗ logrel (Load e).
+  Proof.
+    iIntros "#IH !#" (vs) "#Henv"; rewrite /interp_expr /=.
+    iApply (wp_bind (fill [LoadCtx])).
+    iApply wp_wand; first by iApply "IH".
+    iIntros (v) "#Hv /=".
+    destruct (val_cases_loc v) as [[? ->]|Hnf].
+    - iApply wp_stuck_weaken.
+      rewrite {2}interp_unfold /=.
+      iDestruct "Hv" as (l) "[% #Hv]"; simplify_eq.
+      iInv (logN .@ l) as (w) "[Hw1 #Hw2]" "Hclose".
+      iApply (wp_load with "Hw1").
+      iNext.
+      iIntros "Hw1". iMod ("Hclose" with "[Hw1 Hw2]"); eauto.
+    - iApply load_stuck; done.
+  Qed.
+
+  Lemma logrel_store e1 e2 : logrel e1 -∗ logrel e2 -∗ logrel (Store e1 e2).
+  Proof.
+    iIntros "#IH1 #IH2 !#" (vs) "#Henv"; rewrite /interp_expr /=.
+    iApply (wp_bind (fill [StoreLCtx _])).
+    iApply wp_wand; first by iApply "IH1".
+    iIntros (v1) "#Hv1 /=".
+    iApply (wp_bind (fill [StoreRCtx _])).
+    iApply wp_wand; first by iApply "IH2".
+    iIntros (v2) "#Hv2 /=".
+    destruct (val_cases_loc v1) as [[? ->]|Hnf].
+    - iApply wp_stuck_weaken.
+      rewrite {3}interp_unfold /=.
+      iDestruct "Hv1" as (l) "[% #Hv1]"; simplify_eq.
+      iInv (logN .@ l) as (w) "[Hw1 #Hw2]" "Hclose".
+      iApply (wp_store with "Hw1").
+      iNext.
+      iIntros "Hw1". iMod ("Hclose" with "[Hw1 Hw2]"); eauto.
+      rewrite {6}interp_unfold /=; done.
+    - iApply store_stuck; done.
+  Qed.
+
+  Lemma logrel_CAS e1 e2 e3 : logrel e1 -∗ logrel e2 -∗ logrel e3 -∗ logrel (CAS e1 e2 e3).
+  Proof.
+    iIntros "#IH1 #IH2 #IH3 !#" (vs) "#Henv"; rewrite /interp_expr /=.
+    iApply (wp_bind (fill [CasLCtx _ _])).
+    iApply wp_wand; first by iApply "IH1".
+    iIntros (v1) "#Hv1 /=".
+    iApply (wp_bind (fill [CasMCtx _ _])).
+    iApply wp_wand; first by iApply "IH2".
+    iIntros (v2) "#Hv2 /=".
+    iApply (wp_bind (fill [CasRCtx _ _])).
+    iApply wp_wand; first by iApply "IH3".
+    iIntros (v3) "#Hv3 /=".
+    destruct (val_cases_loc v1) as [[? ->]|Hnf].
+    - iApply wp_stuck_weaken.
+      rewrite {4}interp_unfold /=.
+      iDestruct "Hv1" as (l) "[% #Hv1]"; simplify_eq.
+      iInv (logN .@ l) as (w) "[Hw1 #Hw2]" "Hclose".
+      destruct (decide (v2 = w)) as [|Hneq]; subst.
+    + iApply (wp_cas_suc with "Hw1"); auto using to_of_val.
+      iNext.
+      iIntros "Hw1". iMod ("Hclose" with "[Hw1 Hw2]"); eauto.
+      rewrite {8}interp_unfold /=; done.
+    + iApply (wp_cas_fail with "Hw1"); auto using to_of_val.
+      iNext.
+      iIntros "Hw1". iMod ("Hclose" with "[Hw1 Hw2]"); eauto.
+      rewrite {8}interp_unfold /=; done.
+    - iApply cas_stuck; done.
+  Qed.
+
+  Lemma logrel_FAA e1 e2 : logrel e1 -∗ logrel e2 -∗ logrel (FAA e1 e2).
+  Proof.
+    iIntros "#IH1 #IH2 !#" (vs) "#Henv"; rewrite /interp_expr /=.
+    iApply (wp_bind (fill [FAALCtx _])).
+    iApply wp_wand; first by iApply "IH1".
+    iIntros (v1) "#Hv1 /=".
+    iApply (wp_bind (fill [FAARCtx _])).
+    iApply wp_wand; first by iApply "IH2".
+    iIntros (v2) "#Hv2 /=".
+    destruct (val_cases_loc v1) as [[? ->]|Hnf];
+      last by iApply faa_stuck_non_loc_or_non_nat; auto.
+    destruct (val_cases_nat v2) as [[? ->]|Hnf];
+      last by iApply faa_stuck_non_loc_or_non_nat; auto.
+    rewrite {3}interp_unfold /=.
+    iDestruct "Hv1" as (l) "[% #Hv1]"; simplify_eq.
+    iInv (logN .@ l) as (w) "[>Hw1 #Hw2]" "Hclose".
+    destruct (val_cases_nat w) as [[? ->]|Hnf].
+    -iApply wp_stuck_weaken.
+     iApply (wp_FAA with "Hw1"); auto using to_of_val.
+     iNext.
+     iIntros "Hw1".
+     iMod ("Hclose" with "[Hw1]"); last by eauto.
+     iNext; iExists _; iFrame.
+     rewrite {6}interp_unfold /=; done.
+    - iApply faa_stuck_non_nat_loc; done.
+  Qed.
+
+  Theorem fundamental e : valid_adversary e → ⊢ logrel e.
+  Proof.
+    induction e; intros Hedv; simpl in *; intuition.
+    - iApply logrel_var; done.
+    - iApply logrel_rec; done.
+    - iApply logrel_app; done.
+    - iApply logrel_lam; done.
+    - iApply logrel_letin; done.
+    - iApply logrel_seq; done.
+    - iApply logrel_unit; done.
+    - iApply logrel_nat; done.
+    - iApply logrel_bool; done.
+    - iApply logrel_nat_binop; done.
+    - iApply logrel_if; done.
+    - iApply logrel_pair; done.
+    - iApply logrel_fst; done.
+    - iApply logrel_snd; done.
+    - iApply logrel_injl; done.
+    - iApply logrel_injr; done.
+    - iApply logrel_case; done.
+    - iApply logrel_fork; done.
+    - iApply logrel_alloc; done.
+    - iApply logrel_load; done.
+    - iApply logrel_store; done.
+    - iApply logrel_CAS; done.
+    - iApply logrel_FAA; done.
+  Qed.
+
+End typed_interp.
