lawyer/nonblocking/logrel/persistent_pred.v
@@ -1,0 +1,52 @@
+From stdpp Require Import tactics.
+From iris.bi Require Import bi.
+From iris.prelude Require Import options.
+
+
+Section persistent_pred.
+  Context (A : Type) (PROP : bi).
+
+  (* The domain of semantic types: persistent Iris predicates type A. *)
+  Record persistent_pred := PersPred {
+    pers_pred_car :> A → PROP;
+    pers_pred_persistent x : Persistent (pers_pred_car x)
+  }.
+  Local Arguments PersPred _%I {_}.
+  Global Existing Instances pers_pred_persistent.
+
+  Local Instance persistent_pred_equiv : Equiv persistent_pred :=
+    λ Φ Φ', ∀ x, Φ x ≡ Φ' x.
+  Local Instance persistent_pred_dist : Dist persistent_pred :=
+    λ n Φ Φ', ∀ x, Φ x ≡{n}≡ Φ' x.
+  Definition persistent_pred_ofe_mixin : OfeMixin persistent_pred.
+  Proof. by apply (iso_ofe_mixin (pers_pred_car : _ → A -d> _)). Qed.
+  Canonical Structure persistent_predO :=
+    Ofe persistent_pred persistent_pred_ofe_mixin.
+
+  Global Instance persistent_pred_cofe : Cofe persistent_predO.
+  Proof.
+    apply (iso_cofe_subtype' (λ Φ : A -d> PROP, ∀ w, Persistent (Φ w))
+      PersPred pers_pred_car)=> //.
+    - apply _.
+    - apply limit_preserving_forall=> w.
+      by apply bi.limit_preserving_Persistent=> n ??.
+  Qed.
+
+  Global Instance persistent_pred_car_ne n :
+    Proper (dist n ==> (=) ==> dist n)
+      pers_pred_car.
+  Proof. by intros ? ? ? ? ? ->. Qed.
+  Global Instance persistent_pred_car_proper :
+    Proper ((≡) ==> (=) ==> (≡)) pers_pred_car.
+  Proof. by intros ? ? ? ? ? ->. Qed.
+
+  Lemma persistent_pred_ext (f g : persistent_pred) : f ≡ g ↔ ∀ x, f x ≡ g x.
+  Proof. done. Qed.
+
+  Global Instance: Inhabited persistent_pred := populate (PersPred (λ _, True))%I.
+
+End persistent_pred.
+
+Global Arguments PersPred {_ _} _%I {_}.
+Global Arguments pers_pred_car {_ _} !_ _.
+Global Instance: Params (@pers_pred_car) 2 := {}.
